RequestProject/Exercises.lean
@@ -13,3 +13,4 @@ import RequestProject.Exercises.PartA
 import RequestProject.Exercises.PartBC
 import RequestProject.Exercises.PartBCAux
 import RequestProject.Exercises.PartBCPCP
+import RequestProject.Exercises.PartBCUnary
